\documentclass{article}
\author{Parham Alvani (9231058)}
\title{DS Problem Set No.2}
\begin{document}
\begin{titlepage}
\begin{center}
\emph{In The Name Of God}
\end{center}
\maketitle
\begin{center}
powered by \LaTeX
\end{center}
\end{titlepage}
\tableofcontents
\newpage
\section{Part 8.1}
Problem 2: Part A)
$$
n = 4 , k = 19 \left(\begin{array}{c}
4+19-1\\
19
\end{array}\right)
=
\left(\begin{array}{c}
21\\
19
\end{array}\right)
$$
Part C)
$$
y_3 = x_3 - 3 \rightarrow  0 \leq y_3 \leq 4
$$
$$
y_4 = x_4 - 3 \rightarrow 0 \leq y_4 \leq 5
$$
$$
c_1 : x_1 > 5
$$
$$
c_2 : x_2 > 6
$$
$$
c_3 : y_3 > 4
$$
$$
c_4 : y_4 > 5
$$
$$
N(\bar{c_1} \bar{c_2} \bar{c_3} \bar{c_4})
$$
$$
=|S|-(N(c_1)+N(c_2)+N(c_3)+N(c_4))+(N(c_1c_2)+N(c_2c_3)+N(c_3c_4)+N(c_1c_3)+N(c_2c_4)+N(c_1c_4))
$$
$$
-(N(c_1c_2c_3)+N(c_1c_3c_4)+N(c_2c_3c_4)+(c_1c_2c_4))+(N(c_1c_2c_3c_4))
$$
$$
=
\left(\begin{array}{c}
21\\
4
\end{array}\right)
-
\left(
\left(\begin{array}{c}
16\\
4
\end{array}\right)
+
\left(\begin{array}{c}
15\\
4
\end{array}\right)
+
\left(\begin{array}{c}
17\\
4
\end{array}\right)
+
\left(\begin{array}{c}
16\\
4
\end{array}\right)
\right)
$$
$$
+
\left(
\left(\begin{array}{c}
10\\
4
\end{array}\right)
+
\left(\begin{array}{c}
12\\
4
\end{array}\right)
+
\left(\begin{array}{c}
11\\
4
\end{array}\right)
+
\left(\begin{array}{c}
11\\
4
\end{array}\right)
+
\left(\begin{array}{c}
10\\
4
\end{array}\right)
+
\left(\begin{array}{c}
12\\
4
\end{array}\right)
\right)
$$
$$
-
\left(
\left(\begin{array}{c}
6\\
4
\end{array}\right)
+
\left(\begin{array}{c}
5\\
4
\end{array}\right)
+
\left(\begin{array}{c}
6\\
4
\end{array}\right)
+
\left(\begin{array}{c}
5\\
4
\end{array}\right)
\right)
+
0
$$
Problem 3:
$$
N=S_0=\frac{11!}{(2!)^3}
$$
$$
N(c_1)=\frac{9!}{(2!)^2}
,
\left(\begin{array}{c}
6\\
1
\end{array}\right)
\left[
\frac{9!}{(2!)^2}
\right]
$$
$$
N(c_1c_2)=N(c_1c_3)=N(c_1c_6)=N(c_2c_4)=N(c_2c_5)=N(c_3c_4)=
$$
$$
N(c_3c_4)=N(c_3c_5)=N(c_4c_6)=N(c_5c_6)=0
$$
$$
N(c_1c_4)=\frac{7!}{2!},S_2=6*\frac{7!}{2!},S_3=S_4=S_5=S_6=0
$$
$$
N(\bar{c_1}\bar{c_2}\bar{c_3}\bar{c_4}\bar{c_5}\bar{c_6})=S_0-S_1+S_2=\frac{11!}{(2!)^3}-
\left(\begin{array}{c}
6\\
1
\end{array}\right)
\left[
\frac{9!}{(2!)^2}
\right]
+
6*\frac{7!}{2!}
$$
Problem 5:
$$
(x_1x_2x_3x_4x_5x_6x_7)_10
\rightarrow
x_1+x_2+\cdots+x_7=31,0\leq x_i \leq 9(1\leq i\leq 7)
$$
$$
\rightarrow
\left(\begin{array}{c}
37\\
31
\end{array}\right)
-
\left(\begin{array}{c}
7\\
1
\end{array}\right)
\left(\begin{array}{c}
27\\
21
\end{array}\right)
+
\left(\begin{array}{c}
7\\
2
\end{array}\right)
\left(\begin{array}{c}
17\\
11
\end{array}\right)
-
\left(\begin{array}{c}
7\\
3
\end{array}\right)
\left(\begin{array}{c}
7\\
1
\end{array}\right)
$$
Problem 8:
$$
x_1+x_2+x_3+x_4=9,1\leq i \leq 4
\rightarrow
\left(\begin{array}{c}
12\\
9
\end{array}\right)
-
\left(\begin{array}{c}
4\\
1
\end{array}\right)
\left(\begin{array}{c}
8\\
5
\end{array}\right)
+
\left(\begin{array}{c}
4\\
2
\end{array}\right)
\left(\begin{array}{c}
4\\
1
\end{array}\right)
$$
Problem 11:
$$
\frac{[6^8
-
\left(\begin{array}{c}
6\\
1
\end{array}\right)
5^8
+
\left(\begin{array}{c}
6\\
2
\end{array}\right)
4^8
-
\left(\begin{array}{c}
6\\
3
\end{array}\right)
3^8
+
\left(\begin{array}{c}
12\\
9
\end{array}\right)
2^8
-
\left(\begin{array}{c}
12\\
9
\end{array}\right)]}
{6^8}
$$
Problem 12:
$$
10^9
-
\left(\begin{array}{c}
3\\
1
\end{array}\right)
(9^9)
+
\left(\begin{array}{c}
3\\
2
\end{array}\right)
(8^9)
-
\left(\begin{array}{c}
3\\
3
\end{array}\right)
(7^9)
$$
Problem 15:
$$
c_i \rightarrow x_i>6
$$
$$
N(\bar{c_1}\bar{c_2}\bar{c_3}\bar{c_4}\bar{c_5})=S_0-S_1+S_2
=
\left(\begin{array}{c}
19\\
15
\end{array}\right)
-
\left(\begin{array}{c}
5\\
1
\end{array}\right)
\left(\begin{array}{c}
13\\
9
\end{array}\right)
+
\left(\begin{array}{c}
5\\
2
\end{array}\right)
\left(\begin{array}{c}
7\\
3
\end{array}\right)
$$
$$
=3876-5*715+10*35
=3876-3575+350=651
$$
and the answer is :
$$
\frac{651}{7776}
=
0.08372
$$
\section{Part 8.2}
Problem 2: Part A)
1.
$$
E_2=S_2
-
\left(\begin{array}{c}
3\\
1
\end{array}\right)
S_3
+
\left(\begin{array}{c}
4\\
2
\end{array}\right)
S_4
=
544320
-
(3)(80640)
+
(6)(5040)
=
332640
$$
2.
$$
L_2=S_2
-
\left(\begin{array}{c}
2\\
1
\end{array}\right)
S_3
+
\left(\begin{array}{c}
3\\
1
\end{array}\right)
S_4
=
398160
$$
Part B)
1.
$$
E_3=S_3-
\left(\begin{array}{c}
4\\
1
\end{array}\right)
S_4
=
60480
$$
2.
$$
L_3=S_3-
\left(\begin{array}{c}
3\\
2
\end{array}\right)
S_4
=
65520
$$
Problem 4:
$$
E_3=S_3-
\left(\begin{array}{c}
4\\
1
\end{array}\right)
S_4
+
\left(\begin{array}{c}
5\\
2
\end{array}\right)
S_5
-
\left(\begin{array}{c}
6\\
3
\end{array}\right)
S_6
+
\left(\begin{array}{c}
7\\
4
\end{array}\right)
S_7
=
\left(\begin{array}{c}
7\\
3
\end{array}\right)
4^{10}
-
\left(\begin{array}{c}
4\\
1
\end{array}\right)
\left(\begin{array}{c}
7\\
4
\end{array}\right)
3^{10}
$$
$$
+
\left(\begin{array}{c}
5\\
2
\end{array}\right)
\left(\begin{array}{c}
7\\
5
\end{array}\right)
2^{10}
-
\left(\begin{array}{c}
6\\
3
\end{array}\right)
\left(\begin{array}{c}
7\\
6
\end{array}\right)
1^{10}
+
\left(\begin{array}{c}
7\\
4
\end{array}\right)
\left(\begin{array}{c}
7\\
7
\end{array}\right)
0^{10}
=
28648200
$$
$$
L_3=S_3-
\left(\begin{array}{c}
3\\
2
\end{array}\right)
S_4
+
\left(\begin{array}{c}
4\\
2
\end{array}\right)
S_5
-
\left(\begin{array}{c}
3\\
2
\end{array}\right)
S_6
+
\left(\begin{array}{c}
6\\
2
\end{array}\right)
S_7
$$
$$
=\left(\begin{array}{c}
7\\
3
\end{array}\right)
4^{10}
-
\left(\begin{array}{c}
3\\
2
\end{array}\right)
\left(\begin{array}{c}
7\\
4
\end{array}\right)
3^{10}
+
\left(\begin{array}{c}
4\\
2
\end{array}\right)
\left(\begin{array}{c}
7\\
5
\end{array}\right)
2^{10}
-
\left(\begin{array}{c}
5\\
2
\end{array}\right)
\left(\begin{array}{c}
7\\
6
\end{array}\right)
1^{10}
$$
Problem 5:
\newline
Problem 7: Part A)
$$
N(\bar{c_1}\bar{c_2}\bar{c_3}\bar{c_4})
=
\left(\begin{array}{c}
52\\
13
\end{array}\right)
-
\left(\begin{array}{c}
4\\
1
\end{array}\right)
\left(\begin{array}{c}
39\\
13
\end{array}\right)
+
\left(\begin{array}{c}
4\\
2
\end{array}\right)
\left(\begin{array}{c}
26\\
13
\end{array}\right)
-
\left(\begin{array}{c}
4\\
3
\end{array}\right)
\left(\begin{array}{c}
13\\
13
\end{array}\right)
$$
and the answer is:
$$
\frac{N(\bar{c_1}\bar{c_2}\bar{c_3}\bar{c_4})
}{\left(\begin{array}{c}
52\\
13
\end{array}\right)
}
$$
Part B)
$$
E_1=S_1
+
\left(\begin{array}{c}
2\\
1
\end{array}\right)
S_2
+
\left(\begin{array}{c}
3\\
2
\end{array}\right)
S_3
-
\left(\begin{array}{c}
4\\
3
\end{array}\right)
S_4
$$
$$
=
\left(\begin{array}{c}
39\\
13
\end{array}\right)
\left(\begin{array}{c}
4\\
1
\end{array}\right)
-
2
\left(\begin{array}{c}
4\\
2
\end{array}\right)
\left(\begin{array}{c}
26\\
13
\end{array}\right)
+
3
\left(\begin{array}{c}
4\\
3
\end{array}\right)
\left(\begin{array}{c}
13\\
13
\end{array}\right)
-0
$$
and the answer is :
$$
E_1
/
\left(\begin{array}{c}
52\\
13
\end{array}\right)
$$
Part C)
$$
E_2=S_2
-
\left(\begin{array}{c}
3\\
1
\end{array}\right)
S_3
=
\left(\begin{array}{c}
4\\
2
\end{array}\right)
\left(\begin{array}{c}
26\\
13
\end{array}\right)
-
3
\left(\begin{array}{c}
13\\
13
\end{array}\right)
\left(\begin{array}{c}
4\\
3
\end{array}\right)
$$
and the answer is:
$$
E_2/
\left(\begin{array}{c}
52\\
13
\end{array}\right)
$$
Problem 8: Part B)
$$
L_{t-1} = L_t + E_{t-1} , E_{t-1} = S_{t-1} - tS_t
$$
Part C)
$$
L_{t-1} = L_t + E_{t-1} = S_t + S_{t-1} - tS_t = S_{t-1} - (t-1)S_t = S_{t-1}
-
\left(\begin{array}{c}
t-1\\
t-2
\end{array}\right)
S_t
$$
Part D)
$$
L_m = L_{m+1} + E_m
$$
Part E)
$$
L_{t-1} = S_{t-1} -
\left(\begin{array}{c}
t-1\\
t-2
\end{array}\right)
S_t
,
L_t = S_t
$$
$$
L_{k+1}=S_{k+1}
-
\left(\begin{array}{c}
k+1\\
k
\end{array}\right)
S_{k+2}
+
\left(\begin{array}{c}
k+2\\
k
\end{array}\right)
S_{k+3}
-
\cdots
+
(-1)^{t-k-1}
\left(\begin{array}{c}
t-1\\
k
\end{array}\right)
S_t
$$
$$
L_k=L_{k+1}+E_k=\left[
S_{k+1}
-
\left(\begin{array}{c}
k+1\\
k
\end{array}\right)
S_{k+2}
+
\left(\begin{array}{c}
k+2\\
k
\end{array}\right)
S_{k+3}
-
\cdots
+
(-1)^{t-k-1}
\left(\begin{array}{c}
t-1\\
k
\end{array}\right)
S_t
\right]
+
$$
$$
\left[
S_{k}
-
\left(\begin{array}{c}
k+1\\
1
\end{array}\right)
S_{k+1}
+
\left(\begin{array}{c}
k+2\\
2
\end{array}\right)
S_{k+2}
-
\cdots
+
(-1)^{t-k}
\left(\begin{array}{c}
t\\
t-k
\end{array}\right)
S_t
\right]
$$
and then we have :
$$
L_k
=
S_k
-
\left(\begin{array}{c}
k\\
k-1
\end{array}\right)
S_{k+1}
+
\left(\begin{array}{c}
k+1\\
k-1
\end{array}\right)
S_{k+2}
-
\cdots
+
(-1)^{t-k}
\left(\begin{array}{c}
t-1\\
k-1
\end{array}\right)
S_t
$$
\section{Part 8.3}
Problem 3:
$$
\left(
1-1+
\frac{1}{2!}
-
\frac{1}{3!}
+
\frac{1}{4!}
-
\frac{1}{5!}
\right)
=
5!
\left(
\frac{1}{2!}
-
\frac{1}{3!}
+
\frac{1}{4!}
-
\frac{1}{5!}
\right)
=
5*4*3
-
5*4
+
5
-
1
=
60-20+5-1=44
$$
Problem 4:
$$
7!
\left(
1-1+
\frac{1}{2!}
-
\frac{1}{3!}
+
\frac{1}{4!}
-
\frac{1}{5!}
+
\frac{1}{6!}
-
\frac{1}{7!}
\right)
=1854
$$
and the answer is :
$$
5040-1854=3186
$$
Problem 5: Part A)
$$
(d_7=(7!)e^{-1})7!-d_7
$$
Part B)
$$
d_{26}
=
(26!)e^{-1}
$$
Problem 8: Part A)
$$
(4!)d_4=(4!)^2e^{-1}
$$
Part B,C)
$$
\frac{2*3^2*6}{(4!)^2e^{-1}}
$$
Problem 10: Part A) 1.
$$
\frac{d_n}{n!}
$$
2.
$$
\frac{n(d_{n-1})}{n!}
$$
3.
$$
1-\frac{d_n}{n!}
$$
4.
$$
\frac{\left(\begin{array}{c}
n\\
r
\end{array}\right)
d_{n-r}}{n!}
$$
Part B) 1.
$$
e^{-1}
$$
2.
$$
e^{-1}
$$
3.
$$
1-e^{-1}
$$
4.
$$
\frac{1}{r!}
*e^{-1}
$$
Problem 11: Part A)
$$
(d_10)^2
$$
Part B)
$$
N(\bar{c_1}\bar{c_2}\cdots\bar{c_{10}})
=
(10!)^2
-
\left(\begin{array}{c}
10\\
1
\end{array}\right)
(9!)^2
+
\left(\begin{array}{c}
10\\
2
\end{array}\right)
(8!)^2
-
\cdots
+
(-1)^{10}
\left(\begin{array}{c}
10\\
0
\end{array}\right)
(0!)^2
$$
Problem 13:
$$
n!
=
\left(\begin{array}{c}
n\\
0
\end{array}\right)
d_0
+
\left(\begin{array}{c}
n\\
1
\end{array}\right)
d_1
+
\left(\begin{array}{c}
n\\
2
\end{array}\right)
d_2
+
\cdots
+
\left(\begin{array}{c}
n\\
n
\end{array}\right)
d_n
=
\sum_{k=0}^{n}
\left(\begin{array}{c}
n\\
k
\end{array}\right)
d_k
$$
Problem 14: Part A)
$$
N(c_i)=(n-1)!
$$
$$
N(c_ic_j)=(n-2)!
$$
$$
N(c_ic_jc_k)=(n-3)!
$$
$$
N(c_1c_2\cdots c_{n-1})=(n-(n-1))!
$$
$$
N(\bar{c_1}\bar{c_2}\cdots\bar{c_{n-1}})=
$$
$$
n!-
\left(\begin{array}{c}
n-1\\
1
\end{array}\right)
(n-1)!
+
\cdots
+
(-1)^k
\left(\begin{array}{c}
n-1\\
k
\end{array}\right)
(n-k)!
+
\cdots
+(-1)^{n-1}
\left(\begin{array}{c}
n-1\\
n-1
\end{array}\right)
(n-(n-1))!
$$
Part B)
$$
d_n+d_{n-1}=
$$
$$
\left[
n!-
\left(\begin{array}{c}
n\\
1
\end{array}\right)
(n-1)!
+
\left(\begin{array}{c}
n\\
2
\end{array}\right)
(n-2)!
-
\cdots
+
(-1)^n
\left(\begin{array}{c}
n\\
n
\end{array}\right)
(n-n)!
\right]
$$
$$
+
\left[
(n-1)!
-
\left(\begin{array}{c}
n-1\\
1
\end{array}\right)
(n-2)!
+
\left(\begin{array}{c}
n-1\\
2
\end{array}\right)
(n-3)!
-
\cdots
+
(-1)^{n-1}
\left(\begin{array}{c}
n-1\\
n-1
\end{array}\right)
((n-1)-(n-1))!
\right]
$$
and then the coefficient of $(n-k)!$ in $d_n+d_{n-1}$ :
$$
(-1)^k
\left(\begin{array}{c}
n\\
k
\end{array}\right)
+
(-1)^{k-1}
\left(\begin{array}{c}
n-1\\
k-1
\end{array}\right)
=
$$
$$
(-1)^{k-1}[[(n-1)!/[(k-1)!(n-k)!]]
-
[n!/[k!(n-k)!]]
$$
$$
=
(-1)^{k-1}
[[k(n-1)!-n!]/[k!(n-k)!]]
$$
$$
=
(-1)^{k-1}
(n-1)!
[(k-n)/[k!(n-k)!]]
$$
$$
(-1)^k(n-1)!/[k!(n-k-1)!]
=
(-1)^k
\left(\begin{array}{c}
n-1\\
k
\end{array}\right)
$$
Problem 15:
$$
\left(\begin{array}{c}
n\\
0
\end{array}\right)
(n-1)!
-
\left(\begin{array}{c}
n\\
1
\end{array}\right)
(n-2)!
+
\left(\begin{array}{c}
n\\
2
\end{array}\right)
(n-3)!
-
\cdots
+
(-1)^{n-1}
\left(\begin{array}{c}
n\\
n-1
\end{array}\right)
(0!)
+
(-1)^{n}
\left(\begin{array}{c}
n\\
n
\end{array}\right)
$$
\section{Supplementary Exercises}
Problem 2:
$$
n_1+n_2+n_3+n_4+n_5+n_6+n_7=37,0\leq n_i \leq 9(1\leq i \leq 6),0\leq n_7 \leq 37
\rightarrow
\left(\begin{array}{c}
43\\
37
\end{array}\right)
-
\left(\begin{array}{c}
6\\
1
\end{array}\right)
\left(\begin{array}{c}
33\\
27
\end{array}\right)
+
\left(\begin{array}{c}
6\\
2
\end{array}\right)
\left(\begin{array}{c}
23\\
17
\end{array}\right)
-
\left(\begin{array}{c}
6\\
3
\end{array}\right)
\left(\begin{array}{c}
13\\
7
\end{array}\right)
=930931
$$
Problem 6: Part A)
$$
N(\bar{c_1}\bar{c_2}\bar{c_3}\bar{c_4}\bar{c_5})
=
k^5
-
\left(\begin{array}{c}
5\\
1
\end{array}\right)
k^4
+
\left(\begin{array}{c}
5\\
2
\end{array}\right)
k^3
-
\left(\begin{array}{c}
5\\
3
\end{array}\right)
k^2
+
\left(\begin{array}{c}
5\\
4
\end{array}\right)
k
-
\left(\begin{array}{c}
5\\
5
\end{array}\right)
k
$$
Part B)
$$
k=1,2 \rightarrow 0,k=3 \rightarrow 30
$$
Part C)
$$
k^6
-
\left(\begin{array}{c}
6\\
1
\end{array}\right)
k^5
+
\left(\begin{array}{c}
6\\
2
\end{array}\right)
k^4
-
\left(\begin{array}{c}
6\\
3
\end{array}\right)
k^3
+
\left(\begin{array}{c}
6\\
4
\end{array}\right)
k^2
-
\left(\begin{array}{c}
6\\
5
\end{array}\right)
k
+
\left(\begin{array}{c}
6\\
6
\end{array}\right)
k
$$
Problem 8:
\newline
Problem 9: Part A)
$$
T=\frac{13!}{(2!)^5}
$$
$$
S_5=
\left(\begin{array}{c}
5\\
5
\end{array}\right)
(8!)
,
S_4=
\left(\begin{array}{c}
5\\
4
\end{array}\right)
\left(
\frac{9!}{2!}
\right)
,
S_3=
\left(\begin{array}{c}
5\\
3
\end{array}\right)
\left[
\frac{10!}{(2!)^2}
\right]
$$
$$
E_3=
\frac{
\left[
S_3+
\left(\begin{array}{c}
4\\
1
\end{array}\right)
S_4
+
\left(\begin{array}{c}
5\\
2
\end{array}\right)
S_5
\right]
}{T}
$$
Part B)
$$
E_5=S_5
,
E_4=[S_4-
\left(\begin{array}{c}
5\\
1
\end{array}\right)
S_5
]
$$
and the answer is:
$$
\frac{[T-(E_4+E_5)]}{T}
$$
Problem 10:
$$
N(\bar{c_1}\bar{c_2}\bar{c_3}\bar{c_4})
=
\frac{16!}{(4!)^2}
-
\left(\begin{array}{c}
4\\
1
\end{array}\right)
\left[
\frac{13!}{(4!)^3}
\right]
+
\left(\begin{array}{c}
4\\
2
\end{array}\right)
\left[
\frac{10!}{(4!)^2}
\right]
-
\left(\begin{array}{c}
4\\
3
\end{array}\right)
\left(
\frac{7!}{4!}
\right)
+
\left(\begin{array}{c}
4\\
4
\end{array}\right)
(4!)
$$
Problem 11: Part A)
$$
\left(\begin{array}{c}
n-m\\
r-m
\end{array}\right)
=
\left(\begin{array}{c}
n-m\\
n-r
\end{array}\right)
$$
Part B)
$$
\left(\begin{array}{c}
n-m\\
n-r
\end{array}\right)
=
N(\bar{c_1}\bar{c_2}\cdots\bar{c_m})
=
\sum_{i=0}^{m}
(-1)^i
\left(\begin{array}{c}
m\\
i
\end{array}\right)
\left(\begin{array}{c}
n-i\\
r
\end{array}\right)
$$
\end{document}