\documentclass{article}
\title{DS Problem Set No.1}
\author{Parham Alvani (9231058)} 
\begin{document}
\begin{titlepage}
\begin{center}
\emph{In The Name of God}
\end{center}
\maketitle
\begin{center}
powered by \LaTeX
\end{center}
\end{titlepage}
\tableofcontents
\newpage
\section{Part 1.1-1.2}
	Problem 4:
	Problem 7:
	$$
	2^9
	$$
	Problem 9: Part A)
	$$
	(14)(12)=168
	$$
	Part B)
	$$
	(14)(12)(6)(18)=18144
	$$
	Part C)
	$$
	(8)(18)(6)(3)(14)(12)(14)(12)=73156608
	$$
	Problem 10:
	$$
	(14)(15!)
	$$
	Problem 15:
	$$
	e\underline{x}e\underline{x}e\underline{x}e\underline{x}e
	\Rightarrow
	4!
	$$
	Problem 16: Part A)
	$$
	40^{25}
	$$
	Part B)
	$$
	40 * 30 * 30 * \cdots * 30 * 30 * 40 = (40^2)(30^{23})
	$$
	Problem 23: Part A)
	$$
	\frac{12!}{3!2!2!2!}
	$$
	Part B)
	$$
	\frac{11!}{3!2!2!2!}
	+
	\frac{11!}{3!2!2!2!}
	$$
	Part C)
	$$
	\left(
	\frac{7!}{2!2!}
	\right)
	\left(
	\frac{6!}{2!3!}
	\right)
	$$
	Problem 24:
	$$
	\frac{6!}{2!}
	+
	\frac{6!}{2!2!}
	+
	\frac{6!}{2!2!}
	=
	\left(
	\frac{6!}{2!}
	\right)
	\left(
	1
	+
	\frac{1}{2}
	+
	\frac{1}{2}
	\right)
	=6!
	$$
	Problem 25:
	$$
	\frac{12!}{4!3!2!3!}=277200
	$$
	Problem 28:
	$$
	\frac{14!}{7!7!}
	=
	\left(\begin{array}{c}
	14\\
	7
	\end{array}\right)	
	$$
	Problem 31:
	Part A-B)
	$$
	12*6*8=576	
	$$
	Problem 32: Part A) 5 Letter reverse word	
	$$
	26*26*26*1*1=26^3
	$$
	6 Letter reverse word
	$$
	26*26*26*1*1*1=26^3
	$$
	Part B)
	$$
	26*25*24=15600
	$$
	Problem 38: Part A)
	$$
	3!
	\left(\begin{array}{c}
	8\\
	2
	\end{array}\right)
	\left(\begin{array}{c}
	6\\
	2
	\end{array}\right)
	\left(\begin{array}{c}
	4\\
	2
	\end{array}\right)
	\left(\begin{array}{c}
	2\\
	2
	\end{array}\right)
	$$
	Part B)$ 7200 $
	\newline
	Part C)$ 5760 $
	\newline
	Problem 39: Part A)
	$$
	10 + 128 + 128^2 = 16522 \mbox{ Blocks}
	,
	8459264 \mbox{ Bytes}
	$$
	Part B)
	$$
	10 + 128 + 128^2 + 128^3 = 2113674 \mbox{ Blocks}
	,
	1082201088 \mbox{ Bytes}
	$$
\section{Part 1.3}
	Problem 4: Part A)
	$$
	2^6-1=63
	$$
	Part B)
	$$
	\left(\begin{array}{c}
	6\\
	3
	\end{array}\right)
	=
	20
	$$
	Part C)
	$$
	\left(\begin{array}{c}
	6\\
	2
	\end{array}\right)
	+
	\left(\begin{array}{c}
	6\\
	4
	\end{array}\right)
	+
	\left(\begin{array}{c}
	6\\
	6
	\end{array}\right)
	=31
	$$
	Part D)
	$$
	\left(\begin{array}{c}
	6\\
	4
	\end{array}\right)
	+
	\left(\begin{array}{c}
	6\\
	5
	\end{array}\right)
	+
	\left(\begin{array}{c}
	6\\
	6
	\end{array}\right)
	=22
	$$
	Problem 6:
	$$
	\left(\begin{array}{c}
	n\\
	2
	\end{array}\right)
	+
	\left(\begin{array}{c}
	n-1\\
	2
	\end{array}\right)
	=
	\left(
	\frac{1}{2}
	\right)
	(n)(n-1)
	+
	\left(
	\frac{1}{2}
	\right)
	(n-1)(n-2)
	$$
	$$
	=
	\left(
	\frac{1}{2}
	\right)
	(n-1)[n+(n-2)]
	=
	\left(
	\frac{1}{2}
	\right)
	(n-1)(2n-2)=(n-1)^2
	$$
	Problem 7:
	Problem 13: Part A)
	$$
	\left(\begin{array}{c}
	12\\
	3
	\end{array}\right)
	\left(\begin{array}{c}
	9\\
	3
	\end{array}\right)
	\left(\begin{array}{c}
	6\\
	3
	\end{array}\right)
	\left(\begin{array}{c}
	3\\
	3
	\end{array}\right)
	=
	\frac{12!}{(3!)^4}
	$$
	Part B)
	$$
	\left(\begin{array}{c}
	12\\
	4
	\end{array}\right)
	\left(\begin{array}{c}
	8\\
	4
	\end{array}\right)
	\left(\begin{array}{c}
	4\\
	2
	\end{array}\right)
	\left(\begin{array}{c}
	2\\
	2
	\end{array}\right)
	=
	\frac{12!}{(4!)^2(2!)^2}
	$$
	Problem 21: Part A)
	$$
	\overbrace{\left(\begin{array}{c}
	10\\
	3
	\end{array}\right)}^{\mbox{three 1,seven 0}}
	+
	\overbrace{\left(\begin{array}{c}
	10\\
	1
	\end{array}\right)
	\left(\begin{array}{c}
	9\\
	2
	\end{array}\right)	
	}^{\mbox{two 1,one 2,seven 0}}
	+
	\overbrace{\left(\begin{array}{c}
	10\\
	1
	\end{array}\right)}^{\mbox{one 3,nine 0}}
	=
	220
	$$
	Part B)
	$$
	\left(\begin{array}{c}
	10\\
	4
	\end{array}\right)
	+
	\left(\begin{array}{c}
	10\\
	2
	\end{array}\right)
	+
	\left(\begin{array}{c}
	10\\
	1
	\end{array}\right)
	\left(\begin{array}{c}
	9\\
	2
	\end{array}\right)
	+
	\left(\begin{array}{c}
	10\\
	1
	\end{array}\right)
	\left(\begin{array}{c}
	9\\
	1
	\end{array}\right)
	=
	705
	$$
	Part C)
	$$
	2^{10}
	*
	\sum_{i=0}^{5}
	\left(\begin{array}{c}
	10\\
	2i
	\end{array}\right)
	$$
	Problem 30:Part A)
	$2^3$
	\newline
	Part B)
	$2^{10}$
	\newline
	Part C)
	$3^{10}$
	\newline
	Part D)
	$4^5$
	\newline
	Part E)
	$4^{10}$
	\newline
	Problem 31:
	$$
	\left(\begin{array}{c}
	2n\\
	n
	\end{array}\right)
	+
	\left(\begin{array}{c}
	2n\\
	n-1
	\end{array}\right)
	=
	\frac{(2n)!}{n!n!}
	+
	\frac{(2n)!}{(n-1)!(n+1)!}
	=
	\frac{(2n)!+(n+1)^2+(2n)!(n)(n+1)}{(n+1)!(n+1)!}
	$$
	$$
	=
	\frac{1}{2}
	*
	\frac{(2n)!(2n+2)(n+1)+(2n)!(n)(2n+2)}{(n+1)!(n+1)!}
	$$
	$$
	=
	\frac{1}{2}
	*
	\frac{(2n)!(2n+2)(2n+1)}{(n+1)!(n+1)!}
	$$
	$$
	=
	\frac{1}{2}
	*
	\frac{(2n+2)!}{(n+1)!(n+1)!}
	$$
	$$
	=
	\frac{1}{2}
	\left(\begin{array}{c}
	2n+2\\
	n+1
	\end{array}\right)
	$$
	Problem 34:
	$$
	(1+2)^{n}=3^n
	$$	
\section{Part 1.4}
	Problem 1: Part A)
	$$
	x_1+x_2+x_3+x_4+x_5=10 \rightarrow
	\left(\begin{array}{c}
	5+10-1\\
	10
	\end{array}\right)
	=
	\left(\begin{array}{c}
	14\\
	10
	\end{array}\right)
	$$
	Part B)
	$$
	x_1+x_2+x_3+x_4+x_5=5 \rightarrow
	\left(\begin{array}{c}
	5+5-1\\
	5
	\end{array}\right)
	=
	\left(\begin{array}{c}
	9\\
	5
	\end{array}\right)
	$$
	Part C)
	$$
	x_1+x_2+x_3+x_4+x_5=10 , x_5 \geq 2
	\rightarrow
	\left(\begin{array}{c}
	5+8-1\\
	8
	\end{array}\right)
	=
	\left(\begin{array}{c}
	12\\
	8
	\end{array}\right)
	$$
	Problem 6:
	$$
	\left(\begin{array}{c}
	22\\
	12
	\end{array}\right)
	\left(\begin{array}{c}
	12\\
	4,4,4
	\end{array}\right)
	$$
	Problem 7: Part A)
	$$
	\left(\begin{array}{c}
	4+32-1\\
	32
	\end{array}\right)
	=
	\left(\begin{array}{c}
	35\\
	32
	\end{array}\right)
	$$
	Part B)
	$$
	\left(\begin{array}{c}
	4+28-1\\
	28
	\end{array}\right)
	=
	\left(\begin{array}{c}
	31\\
	28
	\end{array}\right)
	$$
	Part C)
	$$
	\left(\begin{array}{c}
	4+8-1\\
	8
	\end{array}\right)
	=
	\left(\begin{array}{c}
	11\\
	8
	\end{array}\right)
	$$
	Part D)
	$$
	1
	$$
	Part E)
	$$
	\left(\begin{array}{c}
	4+40-1\\
	40
	\end{array}\right)
	=
	\left(\begin{array}{c}
	43\\
	40
	\end{array}\right)
	$$
	Part F)
	$$
	\left(\begin{array}{c}
	4+28-1\\
	28
	\end{array}\right)
	-
	\left(\begin{array}{c}
	4+3-1\\
	3
	\end{array}\right)
	=
	\left(\begin{array}{c}
	31\\
	28
	\end{array}\right)
	-
	\left(\begin{array}{c}
	6\\
	3
	\end{array}\right)
	$$
	Problem 9:
	$$
	230230 = 
	\left(\begin{array}{c}
	n+20-1\\
	20
	\end{array}\right)
	=
	\left(\begin{array}{c}
	n+19\\
	20
	\end{array}\right)
	\Rightarrow
	n=7
	$$
	Problem 7: Part A)
	$$
	\left(\begin{array}{c}
	10+5-1\\
	5
	\end{array}\right)
	=
	\left(\begin{array}{c}
	14\\
	5
	\end{array}\right)
	$$
	Part B)
	$$
	\left(\begin{array}{c}
	7+5-1\\
	5
	\end{array}\right)
	+
	3
	\left(\begin{array}{c}
	7+4-1\\
	4
	\end{array}\right)
	+
	3
	\left(\begin{array}{c}
	7+3-1\\
	3
	\end{array}\right)
	+
	\left(\begin{array}{c}
	7+2-1\\
	2
	\end{array}\right)
	=
	$$
	$$
	\left(\begin{array}{c}
	11\\
	5
	\end{array}\right)
	+
	3
	\left(\begin{array}{c}
	10\\
	4
	\end{array}\right)
	+
	3
	\left(\begin{array}{c}
	9\\
	3
	\end{array}\right)
	+
	\left(\begin{array}{c}
	8\\
	2
	\end{array}\right)	
	$$
	Problem 12:
	$$
	x_1+x_2+\cdots+x_5<40 \Rightarrow
	x_1+x_2+\cdots+x_5 \leq 39 \Rightarrow
	x_1+x_2+\cdots+x_6=39 
	$$
	$$	
	\rightarrow
	\left(\begin{array}{c}
	6+39-1\\
	39
	\end{array}\right)
	=
	\left(\begin{array}{c}
	44\\
	39
	\end{array}\right)
	$$
	Problem 15:
	$$
	x_1+x_2+x_3+x_4=24,1 \leq x_i
	\rightarrow
	\left(\begin{array}{c}
	4+20-1\\
	20
	\end{array}\right)
	=
	\left(\begin{array}{c}
	23\\
	20
	\end{array}\right)	
	$$
	and answer is :
	$$
	(24!)
	\left(\begin{array}{c}
	23\\
	20
	\end{array}\right)
	$$
	Problem 20: Part A)
	$$
	x_1+x_2+x_3=6 \rightarrow
	\left(\begin{array}{c}
	3+6-1\\
	6
	\end{array}\right)
	=
	\left(\begin{array}{c}
	8\\
	6
	\end{array}\right)
	$$
	$$
	x_4+x_5+x_6+x_7=31 \rightarrow
	\left(\begin{array}{c}
	4+31-1\\
	31
	\end{array}\right)
	\left(\begin{array}{c}
	34\\
	31
	\end{array}\right)
	$$
	and answer is :
	$$
	\left(\begin{array}{c}
	8\\
	6
	\end{array}\right)
	\left(\begin{array}{c}
	34\\
	31
	\end{array}\right)
	$$
	Part B)
	$$
	\left(\begin{array}{c}
	5\\
	3
	\end{array}\right)
	\left(\begin{array}{c}
	34\\
	31
	\end{array}\right)
	$$
	Problem 24:
	$$
	\left(\begin{array}{c}
	n+2\\
	3
	\end{array}\right)
	=
	\sum_{i=1}^{i+1}
	\left(\begin{array}{c}
	i+1\\
	2
	\end{array}\right)
	\Rightarrow
	\frac{(n+2)(n+1)n}{6}
	=
	\frac{1}{2}
	\sum_{i=1}^{n}(i+1)i
	\Rightarrow
	$$
	$$
	\frac{(n+2)(n+1)n}{6}
	=
	\frac{1}{2}
	\sum_{i=1}^{n}
	i^2
	+
	\frac{1}{2}
	\sum_{i=1}^{n}
	i
	\Rightarrow
	\frac{1}{2}
	\sum_{i=1}^{n}
	i^2
	=
	\frac{(n+2)(n+1)n}{6}
	-
	\frac{(n+1)n}{4}
	\Rightarrow
	$$
	$$
	\sum_{i=1}^{n}
	i^2
	=
	n(n+1)
	\left[
	\frac{n+2}{3}
	-
	\frac{1}{2}
	\right]
	=
	n(n+1)
	\left[
	\frac{2n+4-3}{6}
	\right]
	=
	\frac{n(n+1)(2n+1)}{6}
	$$
	Problem 25: Part A)
	take above C language program :								
	$sum = 0$
	\newline
	$int i,j,k,m;$
	\newline
	\hspace*{10pt} $for(i=1;i<=n;i++)$
	\newline
	\hspace*{20pt} $for(j=1;j<=i;j++)$
	\newline
	\hspace*{30pt} $for(k=1;k<=j;k++)$
	\newline
	\hspace*{40pt} $for(m=1;m<=k;m++)$
	\newline
	\hspace*{50pt} $sum++;$
	\newline
	after this command rum value of sum equal to
	$$
	\left(\begin{array}{c}
	n+3\\
	4
	\end{array}\right)
	=
	\sum_{i=1}^{n}
	\left(\begin{array}{c}
	i+2\\
	3
	\end{array}\right)
	$$
	Part B)
	$$
	(1)
	\left(\begin{array}{c}
	n+3\\
	4
	\end{array}\right)
	=
	\sum_{i=1}^{n}
	\left(\begin{array}{c}
	i+2\\
	3
	\end{array}\right)
	$$
	$$
	(2)
	\left(
	\frac{1}{4!}
	\right)
	(n+3)(n+2)(n+1)(n)
	=
	\sum_{i=1}^{n}
	\left(
	\frac{1}{6}
	\right)
	(i+2)(i+1)(i)
	$$
	$$
	(3)
	\left(
	\frac{1}{4}
	\right)
	(n+3)(n+2)(n+1)(n)
	=
	\sum_{i=1}^{n}
	(i^3+3i^2+2i)
	$$
	$$
	(4)
	\left(
	\frac{1}{4}
	\right)
	(n+3)(n+2)(n+1)(n)
	=
	\sum_{i=1}^{n}
	i^3
	+
	(3)
	\left(
	\frac{1}{6}
	\right)
	(n)(n+1)(2n+1)
	+
	(2)
	\left(
	\frac{1}{2}
	\right)
	(n+1)(n)
	$$
	$$
	(5)
	\left(
	\frac{1}{4}
	\right)
	(n+1)(n)[(n+3)(n+2)-2(2n+1)-4]
	=
	\sum_{i=1}^{n} i^3
	$$
	$$
	(6)
	\left(
	\frac{1}{4}
	\right)
	(n+1)(n)[n^2+5n+6-4n-6]
	=
	\sum_{i=1}^{n} i^3
	$$
	$$
	(7)
	\left(
	\frac{1}{4}
	\right)
	(n+1)^2(n)^2
	=
	\sum_{i=1}^{n} i^3
	$$
	Problem 26:
	$$
	(r)(r+1)(r+2)\cdots(r+n-1)
	=
	P(r+n-1,r-1)
	$$
	Problem 27: Part A)
	put 1 object in every containers
	$$
	\left(\begin{array}{c}
	n+(m-n)-1\\
	m-n
	\end{array}\right)
	=
	\left(\begin{array}{c}
	m-1\\
	m-n
	\end{array}\right)
	=
	\left(\begin{array}{c}
	m-1\\
	n-1
	\end{array}\right)
	$$
	Part B)
	put r objects in every containers
	$$
	\left(\begin{array}{c}
	n+(m-rn)-1\\
	m-rn
	\end{array}\right)
	=
	\left(\begin{array}{c}
	m-1+(1-r)n\\
	m-rn
	\end{array}\right)
	=
	\left(\begin{array}{c}
	m-1+(1-r)n\\
	n-1
	\end{array}\right)
	$$
\section{Supplementary Exercises}
	Problem 4: Part A)
	$$
	\overbrace{\left(\begin{array}{c}
	25\\
	2
	\end{array}\right)}^{\mbox{Book 1}}\cdots\overbrace{\left(\begin{array}{c}
	25\\
	2	
	\end{array}\right)}^{\mbox{Book 3}}=300*300*300
	$$
	Part B)
	$$
	3\left(\begin{array}{c}
	25\\
	1
	\end{array}\right)^2
	\left(\begin{array}{c}
	25\\
	4
	\end{array}\right)
	+
	6\left(\begin{array}{c}
	25\\
	1
	\end{array}\right)
	\left(\begin{array}{c}
	25\\
	2
	\end{array}\right)
	\left(\begin{array}{c}
	25\\
	3	
	\end{array}\right)
	+
	\left(\begin{array}{c}
	25\\
	2
	\end{array}\right)^3
	$$
	Problem 6:
	$$
	x_1+x_2+x_3+\cdots+x_{15}+x_{16}=45 \quad x_1\geq{0},x_{16}\geq{0} \quad (2\leq{i}\leq{15}),x_i>0
	$$
	$$
	y_1+y_2+y_3+\cdots+y_{15}+y_{16}=31 \quad (1\leq{i}\leq{16}),y_i\geq{0}	
	$$
	$$
	\left(\begin{array}{c}
	16+31-1\\
	31
	\end{array}\right)
	=
	\left(\begin{array}{c}
	46\\
	15
	\end{array}\right)
	$$
	Problem 11: Part A)
	$$
	2+4+1+5=12
	$$
	Part B)
	$$
	2+4+5+8+10+20=49
	$$
	Problem 15: Part A) 1.	
	$$
	\left(\begin{array}{c}
	5\\
	4
	\end{array}\right)
	+
	\left(\begin{array}{c}
	5\\
	2
	\end{array}\right)
	\left(\begin{array}{c}
	4\\
	2
	\end{array}\right)
	+
	\left(\begin{array}{c}
	4\\
	4
	\end{array}\right)
	$$
	2.
	$$
	\left(\begin{array}{c}
	5+4-1\\
	4
	\end{array}\right)
	+
	\left(\begin{array}{c}
	5+2-1\\
	2
	\end{array}\right)
	\left(\begin{array}{c}
	4+2-1\\
	2
	\end{array}\right)
	+
	\left(\begin{array}{c}
	4+4-1\\
	4
	\end{array}\right)
	=
	\left(\begin{array}{c}
	8\\
	4
	\end{array}\right)
	+
	\left(\begin{array}{c}
	6\\
	2
	\end{array}\right)
	\left(\begin{array}{c}
	5\\
	2
	\end{array}\right)
	+
	\left(\begin{array}{c}
	7\\
	4
	\end{array}\right)
	$$
	3.
	$$
	\left(\begin{array}{c}
	8\\
	4
	\end{array}\right)
	+
	\left(\begin{array}{c}
	6\\
	2
	\end{array}\right)
	\left(\begin{array}{c}
	5\\
	2
	\end{array}\right)
	+
	\left(\begin{array}{c}
	7\\
	4
	\end{array}\right)
	-
	9
	$$
	Part B) 1.
	$$
	\left(\begin{array}{c}
	5\\
	1
	\end{array}\right)
	\left(\begin{array}{c}
	4\\
	3
	\end{array}\right)
	+
	\left(\begin{array}{c}
	5\\
	3
	\end{array}\right)
	\left(\begin{array}{c}
	4\\
	1
	\end{array}\right)
	$$
	2-3.
	$$
	\left(\begin{array}{c}
	5\\
	1
	\end{array}\right)
	\left(\begin{array}{c}
	4+3-1\\
	3
	\end{array}\right)
	+
	\left(\begin{array}{c}
	5+3-1\\
	3
	\end{array}\right)
	\left(\begin{array}{c}
	4\\
	1
	\end{array}\right)
	=
	\left(\begin{array}{c}
	5\\
	1
	\end{array}\right)
	\left(\begin{array}{c}
	6\\
	3
	\end{array}\right)
	+
	\left(\begin{array}{c}
	7\\
	3
	\end{array}\right)
	\left(\begin{array}{c}
	4\\
	1
	\end{array}\right)
	$$
	Problem 17: Part A)
	$$
	2	
	\left(\begin{array}{c}
	9\\
	4
	\end{array}\right)
	+
	\left(\begin{array}{c}
	9\\
	3
	\end{array}\right)
	$$
	Part B)
	$$
	\left(\begin{array}{c}
	9+4-1\\
	4
	\end{array}\right)
	=
	\left(\begin{array}{c}
	12\\
	4
	\end{array}\right)
	$$
	$$
	2
	\left(\begin{array}{c}
	12\\
	4
	\end{array}\right)
	-
	9
	$$
	Problem 19: Part A)
	$$
	5*(9!)
	$$
	Part B)
	$$
	3*(8!)
	$$
	Problem 20: Part A)
	$$
	x_1+x_2+x_3=6 \rightarrow
	\left(\begin{array}{c}
	3+6-1\\
	6
	\end{array}\right)
	=
	\left(\begin{array}{c}
	8\\
	6
	\end{array}\right)
	$$
	$$
	x_1+x_2+x_3+x_4+x_5=15 \rightarrow \left\lbrace\begin{array}{c}
	x_1+x_2+x_3=6\\
	x_4+x_5=9
	\end{array}	\right.
	$$
	$$
	x_4+x_5=9 \rightarrow
	\left(\begin{array}{c}
	2+9-1\\
	9
	\end{array}\right)
	=
	\left(\begin{array}{c}
	10\\
	9
	\end{array}\right)
	$$
	and answer is :
	$$
	\left(\begin{array}{c}
	10\\
	9
	\end{array}\right)
	\left(\begin{array}{c}
	8\\
	6
	\end{array}\right)
	$$
	Part B) define $0 \leq k \leq 6$
	$$
	x_1+x_2+x_3=k \rightarrow
	\left(\begin{array}{c}
	3+k-1\\
	k
	\end{array}\right)
	=
	\left(\begin{array}{c}
	k+2\\
	k
	\end{array}\right)
	$$
	$$
	x_4+x_5 \leq 15-k \rightarrow
	\left(\begin{array}{c}
	3+15-k-1\\
	15-k
	\end{array}\right)
	=
	\left(\begin{array}{c}
	17-k\\
	15-k
	\end{array}\right)
	$$
	and answer is :
	$$
	\sum_{k=0}^{6}
	\left(\begin{array}{c}
	k+2\\
	k
	\end{array}\right)
	\left(\begin{array}{c}
	17-k\\
	15-k
	\end{array}\right)
	$$
	Problem 23:
	$$
	\frac{2(n+r-k-1}{(n-k)!(r-1)!}
	+
	\frac{(n+r-k-1)!}{(n-k)!(r-2)!}
	$$
	Problem 33: Part A)
	$$
	\frac{11!}{4!7!}
	$$
	Part B)
	$$
	\left(
	\frac{11!}{7!4!}
	\right)
	-
	\left(
	\frac{4!}{2!2!}
	\right)
	\left(
	\frac{4!}{3!1!}
	\right)
	$$
	Part C) 1.
	$$
	\left(
	\frac{11!}{7!4!}
	\right)
	+
	\left(
	\frac{10!}{6!3!1!}
	\right)
	+
	\left(
	\frac{9!}{5!2!2!}
	\right)
	+
	\left(
	\frac{8!}{4!1!3!}
	\right)
	+
	\left(
	\frac{7!}{3!0!4!}
	\right)	
	$$
	2.
	$$
	\left[
	\left(
	\frac{11!}{7!4!}
	\right)
	+
	\left(
	\frac{10!}{6!3!1!}
	\right)
	+
	\left(
	\frac{9!}{5!2!2!}
	\right)
	+
	\left(
	\frac{8!}{4!1!3!}
	\right)
	+
	\left(
	\frac{7!}{3!0!4!}
	\right)
	\right]
	-
	$$
	$$
	\left\lbrace
	\left[
	\left(
	\frac{4!}{2!2!}
	\right)
	+
	\left(
	\frac{3!}{1!1!1!}
	\right)
	+
	\left(
	\frac{2!}{2!}
	\right)
	\right]
	*
	\left[
	\left(
	\frac{4!}{3!1!}
	\right)
	+
	\left(
	\frac{4!}{3!1!}
	\right)
	+
	\left(
	\frac{3!}{2!1!}
	\right)
	\right]
	\right\rbrace
	$$
	Problem 34: Part A)
	$$
	\frac{7!}{4!3!}=35
	$$
	Part B)
	$$
	\frac{7!}{6!1!}=7
	$$
	Part C)
	$$
	35-7=28
	$$
	Part D)
	$$
	\left(\begin{array}{c}
	7\\
	4
	\end{array}\right)
	-
	\left(\begin{array}{c}
	7\\
	5
	\end{array}\right)
	=
	35-21
	$$
	Part E)
	\newline
	$(m,n) \rightarrow (m+1,n+1) $,if the (n+1)-st ballot is for first student.
	\newline
	$(m.n) \rightarrow (m+1,n-1) $,if the (n+1)-st ballot is for second student.
	$$
	\left(\begin{array}{c}
	13\\
	8
	\end{array}\right)
	-
	\left(\begin{array}{c}
	13\\
	9
	\end{array}\right)
	$$ 
\end{document}
